Properly generated code for normalization and relaxation.

PDDL_Checker_Utils.thy
@@ -10,14 +10,14 @@ abbreviation "wf_problem_x P \<equiv>
   let D = domain P in
   ast_problem.wf_problem' P (ast_domain.STG D) (ast_domain.mp_constT D) (ast_problem.mp_objT P)"
 
-abbreviation "enab_exec_x P pa s \<equiv>
-  let D = domain P in  
-  ast_problem.en_exE2 P (ast_domain.STG D) (ast_problem.mp_objT P) pa s"
-
 (* this just directly displays the first error if applicable *)
 fun reveal_error :: "(unit \<Rightarrow> char list \<Rightarrow> char list) + 'a \<Rightarrow> char list + 'a" where
   "reveal_error (Inl e) = Inl (e () [])" |
   "reveal_error (Inr x) = Inr x"
+
+abbreviation "enab_exec_x P pa s \<equiv>
+  let D = domain P in reveal_error( 
+  ast_problem.en_exE2 P (ast_domain.STG D) (ast_problem.mp_objT P) pa s)"
 
 abbreviation "check_wf_domain_x D \<equiv> reveal_error (
   check_wf_domain D (ast_domain.STG D) (ast_domain.mp_constT D))"
@@ -28,6 +28,9 @@ abbreviation "valid_plan_x P \<pi>s \<equiv>
       obT = ast_problem.mp_objT P;
       i = ast_problem.I P in
   reveal_error (ast_problem.valid_plan_fromE P stg obT 1 i \<pi>s)"
+
+
+
 
 
 end
