Precondition_Normalization.thy
@@ -1,44 +1,72 @@
 theory Precondition_Normalization
 imports "AI_Planning_Languages_Semantics.PDDL_STRIPS_Semantics"
-    Type_Normalization Utils AbLa_alts DNF
+    String_Shenanigans AbLa_alts DNF
 begin
+
+(*
+This part helps ensure that names of the split actions are unique.
+This part calculates the DNF for every precondition, only to then discard them again,
+before they are later recalculated... TODO This should probably be cached using Let. *)
+definition "n_clauses ac \<equiv> length (dnf_list (ast_action_schema.precondition ac))"
 
 context ast_domain begin
 
-fun set_pre :: "ast_action_schema \<Rightarrow> term atom formula \<Rightarrow> ast_action_schema" where
-  "set_pre (Action_Schema n params _ eff) pre = Action_Schema n params pre eff"
+definition "max_n_clauses \<equiv> Max (set (map n_clauses (actions D)))"
+definition "prefix_padding \<equiv> max_length (distinct_strings max_n_clauses) + 1"
+
+fun (in -)set_n_pre :: " ast_action_schema \<Rightarrow> string \<Rightarrow> term atom formula \<Rightarrow> ast_action_schema" where
+  "set_n_pre (Action_Schema _ params _ eff) n pre
+  = Action_Schema n params pre eff"
+
+
+definition "split_ac_names ac n \<equiv>
+  map (\<lambda>prefix. pad prefix_padding prefix @ ac_name ac) (distinct_strings n)"
+
 
 fun split_ac :: "ast_action_schema \<Rightarrow> ast_action_schema list" where
   "split_ac ac =
-    map (set_pre ac) (dnf_list (ac_pre ac))"
+    (let clauses = dnf_list (ac_pre ac) in
+    map2 (set_n_pre ac) (split_ac_names ac (length clauses)) clauses)"
 
 definition "split_acs \<equiv> concat (map split_ac (actions D))"
 
-abbreviation "ac_names \<equiv> map ac_name (actions D)"
-
-definition "dummy_ac_names clauses \<equiv>
-  (map ((@) (safe_prefix ac_names)) (distinct_strings (length clauses)))"
-
-definition "dummy_acs g \<equiv>
-  map dummy_ac (zip (dnf_list g) (dummy_ac_names (dnf_list g)))"
-
-end
-
-context ast_problem begin
-
-definition "fmla_normed_dom \<equiv>
+definition "split_dom \<equiv>
   Domain
     (types D)
-    (dummy_pred_decl # predicates D)
+    (predicates D)
     (consts D)
     split_acs"
 
+definition (in ast_problem) "split_prob \<equiv>
+  Problem
+    split_dom
+    (objects P)
+    (init P)
+    (goal P)"
 
-definition "fmla_normed_prob \<equiv>
-  Problem fmla_normed_dom (objects P) (init P) (goal P)" (* TODO dummy goal *)
+
+(* it's important to be able to convert a plan for the output problem into a plan for the input problem.
+  The other direction is probably (hopefully?) not important. *)
+
+fun restore_pa_split where
+  "restore_pa_split (PAction n args) = PAction (drop prefix_padding n) args"
+abbreviation "restore_plan_split \<pi>s \<equiv> map restore_pa_split \<pi>s"
+
 
 end
 
+subsection \<open> Code Setup \<close>
 
+lemmas precond_norm_code =
+  n_clauses_def
+  ast_domain.max_n_clauses_def
+  ast_domain.prefix_padding_def
+  ast_domain.split_ac_names_def
+  ast_domain.split_ac.simps
+  ast_domain.split_acs_def
+  ast_domain.split_dom_def
+  ast_problem.split_prob_def
+  ast_domain.restore_pa_split.simps
+declare precond_norm_code[code]
 
 end
