PDDL_Relaxation.thy
@@ -1,13 +1,15 @@
 theory PDDL_Relaxation
 imports "AI_Planning_Languages_Semantics.PDDL_STRIPS_Semantics"
-    Formula_Normalization Utils AbLa_alts
+    Utils AbLa_alts
 begin
 
 (* This is only defined for pure conjunctive clauses. *)
 fun remove_neg_lits :: "'a formula \<Rightarrow> 'a formula" where
+  "remove_neg_lits (Atom a) = Atom a" |
   "remove_neg_lits (\<^bold>\<not>\<bottom>) = (\<^bold>\<not>\<bottom>)" |
   "remove_neg_lits (Atom a \<^bold>\<and> c) = (Atom a \<^bold>\<and> remove_neg_lits c)" |
-  "remove_neg_lits (\<^bold>\<not>(Atom a) \<^bold>\<and> c) = remove_neg_lits c"
+  "remove_neg_lits (\<^bold>\<not>(Atom a) \<^bold>\<and> c) = remove_neg_lits c" |
+  "remove_neg_lits _ = undefined"
 
 fun relax_eff :: "'a ast_effect \<Rightarrow> 'a ast_effect" where
   "relax_eff (Effect a b) = Effect a []"
@@ -16,39 +18,27 @@ fun relax_ac :: "ast_action_schema \<Rightarrow> ast_action_schema" where
   "relax_ac (Action_Schema n params pre eff) =
     Action_Schema n params (remove_neg_lits pre) (relax_eff eff)"
 
+definition (in ast_domain) "relax_dom \<equiv>
+  Domain
+    (types D)
+    (predicates D)
+    (consts D)
+    (map relax_ac (actions D))"
 
+definition (in ast_problem) "relax_prob \<equiv>
+  Problem
+    relax_dom
+    (objects P)
+    (init P)
+    (remove_neg_lits (goal P))"
 
+subsection \<open> Code Setup \<close>
 
+lemmas relax_code =
+  ast_domain.relax_dom_def
+  ast_problem.relax_prob_def
 
-
-(* TODO: reevaluate the rest: *)
-
-context wf_ast_domain begin
-                          
-fun relaxed_ac :: "ast_action_schema \<Rightarrow> bool" where
-  "relaxed_ac (Action_Schema nam params pre effs) \<longleftrightarrow>
-    (dels effs = [] \<and> is_STRIPS_fmla pre)"
-
-definition "relaxed_dom \<equiv>
-  list_all1 relaxed_ac (actions D)"
-end
-
-context wf_ast_problem begin
-
-definition "relaxed_prob \<equiv>
-  relaxed_dom \<and>
-  is_STRIPS_fmla (goal P)"
-end
-
-locale relaxed_domain = wf_ast_domain +
-  assumes relaxed_dom: relaxed_dom
-
-locale relaxed_problem = wf_ast_problem +
-  assumes relaxed_prob: relaxed_prob
-
-sublocale relaxed_problem \<subseteq> relaxed_domain D
-  using relaxed_prob relaxed_prob_def by (unfold_locales) simp
-
+declare relax_code [code]
 
 
 end
